Make EAE better.

theories/EAE.v
@@ -6,12 +6,6 @@ Require Import paco2 SimF Fresh.
 Set Implicit Arguments.
 Unset Printing Records.
 
-Function list_to_stmt (xl: list var) (Y : list op) (s : stmt) : stmt :=
-  match xl, Y with
-    | x::xl, e :: Y => stmtLet x  (Operation e) (list_to_stmt xl Y s)
-    | _, _ => s
-  end.
-
 Section MapUpdate.
   Open Scope fmap_scope.
   Variable X : Type.
@@ -49,40 +43,50 @@ Section MapUpdate.
   Qed.
 End MapUpdate.
 
+Fixpoint list_to_stmt (xl: list var) (Y : list op) (s : stmt) : stmt :=
+  match xl, Y with
+  | x::xl, e :: Y => stmtLet x  (Operation e) (list_to_stmt xl Y s)
+  | _, _ => s
+  end.
+
+Require Import Filter.
 
 Lemma list_to_stmt_correct L E s xl Y vl
 : length xl = length Y
   -> omap (op_eval E) Y = Some vl
   -> unique xl
   -> disj (of_list xl) (list_union (List.map Op.freeVars Y))
-  -> star2 F.step (L, E, list_to_stmt xl Y s) nil (L, update_with_list' xl (List.map Some vl) E, s).
+  -> star2 F.step (L, E, list_to_stmt xl Y s) nil
+          (L, update_with_list' xl (List.map Some vl) E, s).
 Proof.
-  intros. eapply length_length_eq in H.
-  general induction H; simpl in * |- *.
-  - eapply star2_refl.
-  - monad_inv H0.
-    econstructor 2 with (y:=EvtTau).
+  intros Len Eq Uni Disj.
+  length_equify.
+  general induction Len; simpl in * |- *; eauto using star2_refl.
+  - simpl in *. monad_inv Eq.
+    eapply star2_silent.
     econstructor; eauto.
-    simpl. eapply IHlength_eq; eauto.
-    + eapply omap_op_eval_agree; [|eauto].
-      symmetry. eapply agree_on_update_dead; [|reflexivity].
-      rewrite list_union_start_swap in H2.
-      intro. eapply (H2 x); eauto; cset_tac.
-    + rewrite list_union_start_swap in H2.
-      eapply disj_1_incl; [ eapply disj_2_incl |]; eauto with cset.
+    rewrite list_union_start_swap in Disj.
+    eapply IHLen; eauto.
+    eapply omap_op_eval_agree; eauto.
+    symmetry. eapply agree_on_update_dead; [|reflexivity].
+    eauto with cset.
+    eapply disj_1_incl; [ eapply disj_2_incl |]; eauto with cset.
 Qed.
 
-Lemma list_to_stmt_crash L E s xl Y
+Lemma list_to_stmt_crash L E xl Y s
 : length xl = length Y
   -> omap (op_eval E) Y = None
   -> unique xl
   -> disj (of_list xl) (list_union (List.map Op.freeVars Y))
-  -> exists σ, star2 F.step (L, E, list_to_stmt xl Y s) nil σ /\ state_result σ = None /\ normal2 F.step σ.
+  -> exists σ, star2 F.step (L, E, list_to_stmt xl Y s) nil σ
+         /\ state_result σ = None
+         /\ normal2 F.step σ.
 Proof.
   intros. eapply length_length_eq in H.
   general induction H; simpl in * |- *.
   - monad_inv H0.
-    + eexists; repeat split; eauto using star2_refl. stuck2.
+    + eexists. split. eapply star2_refl.
+      split; eauto. stuck2.
     + rewrite list_union_start_swap in H2.
       edestruct (IHlength_eq L (E [x <- Some x0])); eauto.
       * eapply omap_op_eval_agree; eauto. symmetry.
@@ -90,9 +94,24 @@ Proof.
         intro. eapply (H2 x); cset_tac.
       * eapply disj_1_incl; [ eapply disj_2_incl |]; eauto with cset.
       * dcr. eexists. split; eauto.
-        econstructor 2 with (y:=EvtTau); eauto.
-        econstructor; eauto.
+        eapply star2_silent.
+        econstructor; eauto. eauto.
 Qed.
+
+Fixpoint replace_if X (p:X -> bool) (L:list X) (L':list X) :=
+  match L with
+  | x::L => if p x then
+              match L' with
+              | y::L' => y::replace_if p L L'
+              | _ => nil
+              end
+            else
+              x::replace_if p L L'
+  | _ => nil
+  end.
+
+Local Notation "'IsVar'" := (fun e => B[isVar e]).
+Local Notation "'NotVar'" := (fun e => B[~ isVar e]).
 
 Fixpoint compile s {struct s}
   : stmt  :=
@@ -100,17 +119,12 @@ Fixpoint compile s {struct s}
     | stmtLet x e s => stmtLet x e (compile s)
     | stmtIf x s t => stmtIf x (compile s) (compile t)
     | stmtApp l Y  =>
-      if [ forall n e, get Y n e -> isVar e] then
-        stmtApp l Y
-      else
-        let xl := fresh_list fresh (list_union (List.map Op.freeVars Y)) (length Y) in
-        list_to_stmt xl Y (stmtApp l (List.map Var xl))
+      let Y' := List.filter (fun e => B[~isVar e]) Y in
+      let xl := fresh_list fresh (list_union (List.map Op.freeVars Y)) (length Y') in
+      list_to_stmt xl Y' (stmtApp l (replace_if (fun e => B[~isVar e]) Y (Var ⊝ xl)))
     | stmtReturn x => stmtReturn x
     | stmtFun F t => stmtFun (List.map (fun Zs => (fst Zs, compile (snd Zs))) F) (compile t)
   end.
-
-Definition ParamRel (G:params) (Z Z' : list var) : Prop :=
-  Z = Z' /\ length Z = length G.
 
 Instance SR : ProofRelation params := {
    ParamRel G VL VL' :=   VL = VL' /\ length VL = length G;
@@ -136,64 +150,118 @@ Proof.
   eapply update_unique_commute; eauto; simpl; intuition.
 Qed.
 
+Fixpoint merge_cond (Y:Type) (K:list bool) (L:list Y) (L':list Y) :=
+  match K, L, L' with
+  | true::K, x::L, L' => x::merge_cond K L L'
+  | false::K, L, y::L' => y::merge_cond K L L'
+  | _, _, _ => nil
+  end.
+
+Lemma omap_filter_none X Y (f:X->option Y) (p:X->bool) (L:list X)
+  : omap f (List.filter p L) = None
+    -> omap f L = None.
+Proof.
+  general induction L; intros; simpl in *.
+  cases in H; simpl in *; try monad_inv H.
+  - rewrite H0; simpl; eauto.
+  - rewrite EQ; simpl. erewrite H, IHL; eauto.
+  - destruct (f a); simpl; eauto.
+    erewrite IHL; eauto.
+Qed.
+
+Lemma omap_filter_partitions X Y (f:X->option Y) (p q:X->bool) (L:list X) vl1 vl2
+  : omap f (List.filter p L) = Some vl1
+    -> omap f (List.filter q L) = Some vl2
+    -> (forall n x, get L n x -> negb (p x) = q x)
+    -> omap f L = Some (merge_cond (p ⊝ L) vl1 vl2).
+Proof.
+  general induction L; intros; simpl in *; eauto.
+  cases in H; simpl in *; try monad_inv H.
+  - erewrite <- H1 in H0; eauto using get.
+    rewrite <- Heq in H0. simpl in *.
+    rewrite EQ. simpl.
+    rewrite (IHL _ _ _ _ _ _ EQ1 H0); eauto using get.
+  - erewrite <- H1 in H0; eauto using get.
+    rewrite <- Heq in H0. simpl in *.
+    monad_inv H0. rewrite EQ. simpl.
+    rewrite (IHL _ _ _ _ _ _ H EQ1); eauto using get.
+Qed.
+
+Lemma omap_replace_if V Y Y' vl0 vl1
+  :  omap (op_eval V) (List.filter IsVar Y) = ⎣ vl1 ⎦
+     -> omap (op_eval V) Y' = ⎣ vl0 ⎦
+     -> omap
+         (op_eval V)
+         (replace_if NotVar Y Y') = ⎣ merge_cond (IsVar ⊝ Y) vl1 vl0 ⎦.
+Proof.
+  general induction Y; simpl; eauto.
+  simpl in *. cases in H; cases; isabsurd; simpl in *.
+  - monad_inv H. rewrite EQ. simpl. erewrite IHY; eauto. eauto.
+  - destruct Y'; simpl in *.
+    + inv H0; eauto.
+    + monad_inv H0. rewrite EQ. simpl.
+      erewrite IHY; eauto. simpl; eauto.
+Qed.
 
 Lemma sim_EAE' r L L' V s
-  : simLabenv Bisim r SR (block_Z ⊝ L) L L'
+  : simLabenv Sim r SR (block_Z ⊝ L) L L'
     -> ❬L❭ = ❬L'❭
-    -> sim'r r Bisim (L, V, s) (L',V, compile s).
+    -> sim'r r Sim (L, V, s) (L',V, compile s).
 Proof.
   revert_except s. unfold sim'r.
   sind s; destruct s; simpl; intros; simpl in * |- *.
   - destruct e.
-    + case_eq (op_eval V e); intros.
-      * pone_step; eauto.
-      * pno_step.
-    + case_eq (omap (op_eval V) Y); intros.
-      * pextern_step; eauto.
-      * pno_step.
-  - case_eq (op_eval V e); intros.
-    + case_eq (val2bool v); intros;
-        pone_step; eauto.
-    + pno_step.
-  - case_eq (omap (op_eval V) Y); intros.
-    exploit (list_to_stmt_correct L' V (stmtApp l (Var ⊝ fresh_list fresh (list_union (Op.freeVars ⊝ Y)) ❬Y❭)) (fresh_list fresh (list_union (Op.freeVars ⊝ Y)) ❬Y❭) Y) as LTSC; eauto using fresh_spec, fresh_list_unique, fresh_list_spec.
+    + eapply (sim_let_op il_statetype_F); eauto.
+    + eapply (sim_let_call il_statetype_F); eauto.
+  - eapply (sim_cond il_statetype_F); eauto.
+  - case_eq (omap (op_eval V) (List.filter NotVar Y)); intros.
     + destruct (get_dec L (counted l)) as [[[bE bZ bs n]]|].
       * hnf in H; dcr. inv_get. destruct x as [bE' bZ' bs' n'].
-        decide (length Y = length bZ). {
-          cases.
-          - eapply H3; eauto. hnf; eauto.
-            hnf; eauto with len.
-          - eapply sim'_expansion_closed;
-              [
-              | eapply star2_refl
-              | eapply list_to_stmt_correct;
-                eauto using fresh_spec, fresh_list_unique, fresh_list_spec
-              ]; eauto.
-            simpl. eapply H3; eauto.
-            hnf; eauto.
-            Focus 2.
-            eapply omap_op_eval_agree.
-            eapply update_with_list_agree';
-              eauto using fresh_list_unique, fresh_spec with len.
-            eapply omap_lookup_vars;
-              eauto using fresh_list_unique, fresh_spec with len.
-            hnf; simpl; eauto with len.
-        }
-        cases.
-        pno_step; simpl in *. exploit H3; eauto; dcr; subst. congruence.
-        eapply sim'_expansion_closed; [| eapply star2_refl | eapply LTSC].
-        exploit H3; eauto; dcr. hnf; eauto. simpl in *; dcr; subst.
-        pno_step. simpl in *.
-        eapply n0; rewrite len. rewrite map_length.
-        rewrite fresh_list_length. eauto.
-      * cases. pno_step; eauto. inv_get; eauto.
-        eapply sim'_expansion_closed; [| eapply star2_refl | eapply LTSC].
-        pno_step; repeat get_functional; simpl in *.
-        exploit H; eauto; dcr. inv_get; eauto.
-    + cases. pno_step.
-      edestruct (list_to_stmt_crash L' V (stmtApp l (Var ⊝ fresh_list fresh (list_union (Op.freeVars ⊝ Y)) ❬Y❭)) (fresh_list fresh (list_union (Op.freeVars ⊝ Y)) ❬Y❭) Y); eauto using fresh_spec, fresh_list_unique, fresh_list_spec; dcr.
-      pfold. econstructor 4; [ | eapply star2_refl | eapply H3 | | ]; eauto.
-      stuck2.
+        decide (length Y = length bZ).
+        -- eapply sim'_expansion_closed;
+             [
+             | eapply star2_refl
+             | eapply list_to_stmt_correct;
+               eauto using fresh_spec, fresh_list_unique, fresh_list_spec
+             ]; eauto.
+           ++ case_eq (omap (op_eval V) (List.filter IsVar Y)); intros.
+             ** exploit (omap_filter_partitions _ _ _ H5 H1).
+                intros; repeat cases; eauto.
+                edestruct H3; eauto. hnf; eauto.
+                eapply H9; eauto.
+                hnf. simpl. split; eauto with len.
+                eapply omap_replace_if.
+                erewrite omap_op_eval_agree; eauto.
+                rewrite <-  update_with_list_agree';
+                  eauto using fresh_spec, fresh_list_unique,
+                  fresh_list_spec with len.
+                eapply agree_on_incl.
+                symmetry.
+                eapply update_with_list_agree_minus; eauto.
+                eapply not_incl_minus. reflexivity.
+                symmetry.
+                eapply disj_2_incl.
+                eapply fresh_list_spec; eauto using fresh_spec.
+                eapply list_union_incl; intros; eauto with cset.
+                inv_get. eapply incl_list_union; eauto using map_get_1.
+                eapply omap_op_eval_agree; eauto.
+                Focus 2.
+                eapply omap_lookup_vars; eauto with len.
+                eauto using fresh_spec, fresh_list_unique,
+                fresh_list_spec with len.
+                rewrite <-  update_with_list_agree';
+                  eauto using fresh_spec, fresh_list_unique,
+                  fresh_list_spec with len. reflexivity.
+             ** perr.
+                erewrite omap_filter_none in def; eauto. congruence.
+           ++ eapply disj_2_incl.
+             eapply fresh_list_spec; eauto using fresh_spec.
+             eapply list_union_incl; intros; eauto with cset.
+             inv_get. eapply incl_list_union; eauto using map_get_1.
+        -- perr.
+      * perr.
+    + perr.
+      erewrite omap_filter_none in def; eauto. congruence.
   - pno_step.
   - pone_step.
     left. eapply IH; eauto 20 with len.
@@ -207,25 +275,57 @@ Proof.
 Qed.
 
 Lemma sim_EAE V s
-: @sim _ statetype_F _ statetype_F Bisim (nil, V, s) (nil,V, compile s).
+  : @sim _ statetype_F _ statetype_F Sim (nil, V, s) (nil,V, compile s).
 Proof.
   eapply sim'_sim. eapply sim_EAE'; eauto.
   hnf; intros; split; eauto using @sawtooth with len.
   isabsurd.
 Qed.
 
-Lemma list_to_stmt_app_expfree  ZL Y l ZL'
-  : app_expfree (list_to_stmt ZL Y (stmtApp l (Var ⊝ ZL'))).
+Lemma list_to_stmt_app_expfree  ZL Y Y' l
+  : (forall n e, get Y' n e -> isVar e)
+    -> app_expfree (list_to_stmt ZL Y (stmtApp l Y')).
 Proof.
-  general induction Y; destruct ZL; simpl;
-    econstructor; intros; inv_get; eauto using isVar.
+  general induction Y; destruct ZL; destruct Y'; simpl;
+    econstructor; intros; inv_get; isabsurd; eauto using isVar.
+Qed.
+
+Lemma replace_if_get_inv X (p:X -> bool) L L' n x
+  : get (replace_if p L L') n x
+    -> exists l , get L n l /\
+            ((p l /\ exists l' n', get L' n' l' /\ x = l')
+              \/ (~ p l /\ x = l)).
+Proof.
+  intros; general induction L; destruct L'; simpl in *; isabsurd.
+  - cases in H; isabsurd. inv H.
+    + exists x; split; eauto using get.
+      right; split; eauto. rewrite <- Heq. eauto.
+    + edestruct IHL; eauto; dcr.
+      eexists; split; eauto using get.
+  - cases in H; isabsurd.
+    + inv H.
+      * eexists; split; eauto using get.
+        left. rewrite <- Heq; eauto using get.
+      * edestruct IHL; eauto using get; dcr.
+        eexists; split; eauto using get.
+        destruct H2; dcr; isabsurd. left; eauto 20 using get.
+        right; eauto using get.
+    + inv H.
+      * eexists; split; eauto using get.
+        right. rewrite <- Heq; eauto using get.
+      * edestruct IHL; eauto; dcr.
+        eexists; split; eauto using get.
 Qed.
 
 Lemma EAE_app_expfree s
   : app_expfree (compile s).
 Proof.
   sind s; destruct s; simpl; eauto using app_expfree.
-  - cases; eauto using app_expfree.
-    + eapply list_to_stmt_app_expfree.
+  - eapply list_to_stmt_app_expfree.
+    intros.
+    eapply replace_if_get_inv in H; dcr.
+    destruct H2; dcr; cases in H0; isabsurd; inv_get; eauto using isVar.
+    exfalso; eapply H0; eauto.
+    destruct x; eauto using isVar; exfalso; eapply NOTCOND; intro; isabsurd.
   - econstructor; intros; inv_get; eauto using app_expfree.
 Qed.
